Translate up to context_for_transfer

vfmComputeScript.sml
@@ -1,7 +1,8 @@
 open HolKernel boolLib bossLib Parse dep_rewrite
      cv_typeTheory cv_transLib cv_typeLib
+     cvTheory cv_stdTheory
      pairTheory combinTheory wordsTheory alistTheory arithmeticTheory
-     sptreeTheory vfmExecutionTheory;
+     sptreeTheory vfmContextTheory vfmStateTheory vfmExecutionTheory;
 
 val _ = new_theory "vfmCompute";
 
@@ -61,6 +62,12 @@ Proof
   \\ strip_tac \\ gvs[]
 QED
 
+Theorem build_spt_empty_storage[simp]:
+  ∀n. build_spt 0w n empty_storage = LN
+Proof
+  Induct \\ gvs[build_spt_def, empty_storage_def]
+QED
+
 Definition from_storage_def:
   from_storage (s: storage) =
   from_sptree_sptree_spt ^from_bytes32 (build_spt 0w (dimword (:256)) s)
@@ -112,6 +119,12 @@ Proof
   \\ metis_tac[w2n_lt, NOT_LESS_EQUAL]
 QED
 
+Theorem empty_storage_cv_rep[cv_rep]:
+  from_storage empty_storage = Num 0
+Proof
+  rw[from_storage_def] \\ EVAL_TAC
+QED
+
 val from_to_account_state = from_to_thm_for “:account_state”;
 val to_account_state = from_to_account_state |> concl |> rand;
 val from_account_state = from_to_account_state |> concl |> rator |> rand;
@@ -143,6 +156,67 @@ Proof
   \\ metis_tac[w2n_lt, NOT_LESS_EQUAL]
 QED
 
+val () = cv_auto_trans empty_account_state_def;
+
+val cv_empty_account_state_thm = theorem "cv_empty_account_state_thm";
+
+Definition lookup_account_def:
+  lookup_account (accounts: evm_accounts) address = accounts address
+End
+
+Definition cv_lookup_account_def:
+  cv_lookup_account (a:cv) (k:cv) =
+  let v = cv_lookup k a in
+    cv_if (cv_ispair v) (cv_snd v) (cv_empty_account_state (Num 0))
+End
+
+Theorem lookup_account_cv_rep[cv_rep]:
+  ^from_account_state (lookup_account a k) =
+  cv_lookup_account (from_evm_accounts a) (from_word k)
+Proof
+  gs[lookup_account_def, cv_lookup_account_def, GSYM cv_lookup_thm,
+     from_word_def, from_evm_accounts_def, lookup_build_spt]
+  \\ qspec_then`k`strip_assume_tac w2n_lt
+  \\ simp[]
+  \\ Cases_on`a k = empty_account_state`
+  \\ gs[from_option_def, cv_empty_account_state_thm]
+QED
+
+Definition update_account_def:
+  update_account (accounts: evm_accounts) address new_account =
+    (address =+ new_account) accounts
+End
+
+Definition cv_update_account_def:
+  cv_update_account (a:cv) (k:cv) (v:cv) =
+  cv_if (cv_eq v (cv_empty_account_state (Num 0)))
+    (cv_delete k a)
+    (cv_insert k v a)
+End
+
+Theorem update_account_cv_rep[cv_rep]:
+  from_evm_accounts (update_account a k v) =
+  cv_update_account (from_evm_accounts a) (from_word k) (^from_account_state v)
+Proof
+  gs[from_evm_accounts_def, cv_update_account_def,
+     update_account_def, from_word_def, cv_eq_def]
+  \\ qmatch_goalsub_abbrev_tac`Num (COND ve _ _)`
+  \\ `ve ⇔ v = empty_account_state`
+  by metis_tac[cv_empty_account_state_thm,
+               from_to_account_state,
+               from_to_def]
+  \\ simp[Abbr`ve`]
+  \\ gs[GSYM cv_insert_thm, GSYM cv_delete_thm]
+  \\ IF_CASES_TAC
+  \\ AP_TERM_TAC
+  \\ DEP_REWRITE_TAC[spt_eq_thm]
+  \\ simp[wf_delete, wf_insert, lookup_delete, lookup_insert,
+          lookup_build_spt, APPLY_UPDATE_THM]
+  \\ rw[] \\ gvs[]
+  \\ TRY (qspec_then`k`strip_assume_tac w2n_lt \\ gs[] \\ NO_TAC)
+  \\ qpat_x_assum`_ = empty_account_state`mp_tac \\ rw[] \\ gs[]
+QED
+
 val from_to_transaction_state = from_to_thm_for “:transaction_state”;
 
 val () = “consume_gas n s” |>
@@ -159,14 +233,32 @@ val () = “push_context c s” |>
     COND_RATOR] |>
   cv_auto_trans;
 
+val () = code_for_transfer_def |>
+  ONCE_REWRITE_RULE[GSYM lookup_account_def] |>
+  cv_auto_trans;
+
+Theorem context_for_transfer_unfolded:
+  context_for_transfer ctxt callerAddress incCaller code =
+  ctxt with callParams :=
+    ctxt.callParams with <|
+      accounts := update_account
+        ctxt.callParams.accounts callerAddress incCaller;
+      code := code
+    |>
+Proof
+  rw[context_for_transfer_def,
+     context_component_equality,
+     call_parameters_component_equality,
+     update_account_def]
+QED
+
+val () = cv_auto_trans context_for_transfer_unfolded;
 
 (*
-start_context may need a rewritten version more suited to cv_compute
-
 val () = “start_context x y c s” |>
   SIMP_CONV std_ss [
     start_context_def, bind_def, ignore_bind_def, LET_THM,
-    COND_RATOR, o_THM] |>
+    COND_RATOR] |>
   cv_auto_trans;
 
 val () = cv_auto_trans step_def;
